smtlink/z3_files/test0.py
@@ -1,8 +1,9 @@
 from sys import path
 path.insert(0,"/ubc/cs/home/y/yanpeng/project/ACL2/smtlink/z3_interface")
-from ACL2_translator import to_smt
+from ACL2_translator import to_smt, Q
 s = to_smt()
 X=s.isReal("X")
-hypothesis=True
-conclusion=s.equal(s.plus(X,X),(lambda var0:s.times(2,var0))(X))
+T=("T")
+hypothesis=s.equal(s.plus(X,X),s.times(1,(lambda var0:s.times(2,var0))(X)))
+conclusion=False
 s.prove(hypothesis, conclusion)
