smtlink/z3_files/test3.py
@@ -2,11 +2,8 @@ from sys import path
 path.insert(0,"/ubc/cs/home/y/yanpeng/project/ACL2/smtlink/z3_interface")
 from ACL2_translator import to_smt, Q
 s = to_smt()
+Y=s.isReal("Y")
 =("")
-=("")
-=("")
-=("")
-=("")
-hypothesis=s.lt((lambda var0,var1:s.times(var0,s.plus(1,var1)))(X,Y),(lambda var2,var3:s.times(var2,s.plus(1,var3)))(X,(lambda var4,var5:s.times(var4,s.plus(1,var5)))(X,Z)))
+hypothesis=s.lt(9,(lambda var0:s.times(2,(lambda var1:s.plus(var1,3))(var0)))(Y))
 conclusion=False
 s.prove(hypothesis, conclusion)
