smtlink/test-all.lisp
@@ -2,32 +2,33 @@
 :logic
 
 ;; test0
-(defun bar (x) (* 2 x))
+(defconst *a* 1)
+(defun bar1 (x) (* 2 x))
 
 ;; a very simple theorem
 (defthm test0
   (implies (and (and (rationalp x)) (and))
-	   (equal (+ x x) (bar x)))
+	   (equal (+ x x) (* *a* (bar1 x))))
   :hints
             (("Goal"
               :clause-processor
-              (my-clause-processor clause '((bar) 1 "test0")))))
+              (my-clause-processor clause '((bar1) 1 "test0")))))
 
 ;; test1
-(defun foo (x y) (* x (+ 1 y)))
+(defun foo1 (x y) (* x (+ 1 y)))
 
 ;; very first piece of test case
 (thm (implies (and (and (rationalp x)
 			(integerp y)
 			(integerp z))
 		   (and (not (<= x 0))
-			(equal z (+ 2 4))
-			(or (> x y) (> x (+ y 1)))))
-	      (> (foo x (foo x z)) (foo x y)))
+			(equal z (+ 3/2 4))
+			(or (> x y) (> x (+ y 40/3)))))
+	      (> (foo1 x (foo1 x z)) (foo1 x y)))
      :hints
             (("Goal"
               :clause-processor
-              (my-clause-processor clause '((foo) 2 "test1")))))
+              (my-clause-processor clause '((foo1) 2 "test1")))))
 
 ;; Test cases:
 ;; 1. Without constant definition and function definitions:
@@ -44,180 +45,14 @@
 ;;             (and cond1 cond2 cond3 ...))
 ;;         (concl)
 
+(defun foo (x) (+ x 3))
+(defun bar (y) (* 2 (foo y)))
 
-ACL2 p!>(ld "test-all.lisp")
-
-ACL2 Version 6.4.  Level 2.  Cbd 
-"/ubc/cs/home/y/yanpeng/project/ACL2/smtlink/".
-System books directory 
-"/ubc/cs/research/isd/users/software/ACL2/acl2-sources/books/".
-Type :help for help.
-Type (good-bye) to quit completely out of ACL2.
-
-ACL2 p!>>ACL2 !>>
-Since bar is non-recursive, its admission is trivial.  We observe that
-the type of bar is described by the theorem (acl2-numberp (bar x)).
-We used primitive type reasoning.
-
-Summary
-Form:  ( defun bar ...)
-Rules: ((:fake-rune-for-type-set nil))
-Time:  0.00 seconds (prove: 0.00, print: 0.00, other: 0.00)
- bar
-ACL2 !>>
-ACL2 Warning [Subsume] in ( defthm test0 ...):  The previously added
-rule commutativity-of-+ subsumes a newly proposed :rewrite rule generated
-from test0, in the sense that the old rule rewrites a more general
-target.  Because the new rule will be tried first, it may nonetheless
-find application.
-
-cl: ((implies (if (rationalp x) 't 'nil)
-              (equal (binary-+ x x) (bar x))))
-(bar)
-
- 1
-
- "test0"
-
-The final index number: 1
-(implies (if (rationalp x) 't 'nil)
-         (equal (binary-+ x x)
-                ((lambda (|var0|) (binary-* '2 |var0|))
-                 x)))
-
-proved
-; Z3: `python /ubc/cs/home/y/yanpeng/project/ACL2/smtlink/z3_files/test0.py`:
-0.15 sec, 2,176 bytes
-t
-0
-("proved")
-Success!
- (((not (implies (if (rationalp x) 't 'nil)
-                 (equal (binary-+ x x)
-                        ((lambda (|var0|) (binary-* '2 |var0|))
-                         x))))
-   (implies (if (rationalp x) 't 'nil)
-            (equal (binary-+ x x) (bar x)))))
-
-Goal'
-
-Q.E.D.
-
-Summary
-Form:  ( defthm test0 ...)
-Rules: ((:definition bar)
-        (:definition not)
-        (:executable-counterpart tau-system))
-Hint-events: ((:clause-processor my-clause-processor))
-Warnings:  Subsume
-Time:  0.01 seconds (prove: 0.00, print: 0.00, other: 0.00)
-Prover steps counted:  53
- test0
-ACL2 !>>
-Since foo is non-recursive, its admission is trivial.  We observe that
-the type of foo is described by the theorem (acl2-numberp (foo x y)).
-We used primitive type reasoning.
-
-Summary
-Form:  ( defun foo ...)
-Rules: ((:fake-rune-for-type-set nil))
-Time:  0.00 seconds (prove: 0.00, print: 0.00, other: 0.00)
- foo
-ACL2 !>>cl: ((implies (if (if (rationalp x)
-                      (if (integerp y) (integerp z) 'nil)
-                      'nil)
-                  (if (not (not (< '0 x)))
-                      (if (equal z (binary-+ '2 '4))
-                          (if (< y x)
-                              (< y x)
-                              (< (binary-+ y '1) x))
-                          'nil)
-                      'nil)
-                  'nil)
-              (< (foo x y) (foo x (foo x z)))))
-(foo)
-
- 2
-
- "test1"
-
-The final index number: 6
-(implies (if (if (rationalp x)
-                 (if (integerp y) (integerp z) 'nil)
-                 'nil)
-             (if (not (not (< '0 x)))
-                 (if (equal z (binary-+ '2 '4))
-                     (if (< y x)
-                         (< y x)
-                         (< (binary-+ y '1) x))
-                     'nil)
-                 'nil)
-             'nil)
-         (< ((lambda (|var0| |var1|)
-                     (binary-* |var0| (binary-+ '1 |var1|)))
-             x y)
-            ((lambda (|var2| |var3|)
-                     (binary-* |var2| (binary-+ '1 |var3|)))
-             x
-             ((lambda (|var4| |var5|)
-                      (binary-* |var4| (binary-+ '1 |var5|)))
-              x z))))
-
-proved
-; Z3: `python /ubc/cs/home/y/yanpeng/project/ACL2/smtlink/z3_files/test1.py`:
-0.11 sec, 1,984 bytes
-t
-0
-("proved")
-Success!
- (((not (implies (if (if (rationalp x)
-                         (if (integerp y) (integerp z) 'nil)
-                         'nil)
-                     (if (not (not (< '0 x)))
-                         (if (equal z (binary-+ '2 '4))
-                             (if (< y x)
-                                 (< y x)
-                                 (< (binary-+ y '1) x))
-                             'nil)
-                         'nil)
-                     'nil)
-                 (< ((lambda (|var0| |var1|)
-                             (binary-* |var0| (binary-+ '1 |var1|)))
-                     x y)
-                    ((lambda (|var2| |var3|)
-                             (binary-* |var2| (binary-+ '1 |var3|)))
-                     x
-                     ((lambda (|var4| |var5|)
-                              (binary-* |var4| (binary-+ '1 |var5|)))
-                      x z)))))
-   (implies (if (if (rationalp x)
-                    (if (integerp y) (integerp z) 'nil)
-                    'nil)
-                (if (not (not (< '0 x)))
-                    (if (equal z (binary-+ '2 '4))
-                        (if (< y x)
-                            (< y x)
-                            (< (binary-+ y '1) x))
-                        'nil)
-                    'nil)
-                'nil)
-            (< (foo x y) (foo x (foo x z))))))
-
-Goal'
-Goal''
-
-Q.E.D.
-
-Summary
-Form:  ( THM ...)
-Rules: ((:definition foo)
-        (:definition not)
-        (:executable-counterpart binary-+))
-Hint-events: ((:clause-processor my-clause-processor))
-Time:  0.01 seconds (prove: 0.01, print: 0.00, other: 0.00)
-Prover steps counted:  199
-
-Proof succeeded.
-ACL2 !>>Bye.
- :eof
-ACL2 !>
+(defthm test3
+  (implies (and (and (rationalp y))
+		(and (> y 1)))
+	   (> (bar y) 9))
+  :hints
+  (("Goal"
+    :clause-processor
+    (my-clause-processor clause '((foo bar) 5 "test3")))))
