smtlink/config.lisp
@@ -1,8 +1,9 @@
-0;136;0c;; This file configs the path to below directories:
+;; This file configs the path to below directories:
 ;; 1. Z3_interface
 ;; 2. Z3_files
 ;; 3. name of z3 class
 ;; 4. SMT command
+(in-package "ACL2")
 (defconst *dir-interface* "/ubc/cs/home/y/yanpeng/project/ACL2/smtlink/z3\_interface")
 (defconst *dir-files* "/ubc/cs/home/y/yanpeng/project/ACL2/smtlink/z3\_files")
 (defconst *z3-module* "ACL2\_translator")
