smtlink/helper.lisp
@@ -1,0 +1,7 @@
+;; helper functions for basic data structure manipulation
+(in-package "ACL2")
+
+;; my-last
+(defun my-last (listx)
+ "my-last: fetch the last element from list"
+  (car (last listx)))
