smtlink/z3-hint-raw.lsp
@@ -1,3 +1,4 @@
+(include-book "./helper")
 (include-book "./SMT-formula")
 (include-book "./SMT-translator")
 (include-book "./SMT-run")
@@ -6,7 +7,36 @@
 
 (tshell-ensure)
 
+(mutual-recursion
+;; lisp-code-print-help
+(defun lisp-code-print-help (lisp-code-list)
+  "lisp-code-print-help: make a printable lisp code list, the input parameter is the list of "
+  (if (endp lisp-code-list)
+      nil
+    (list #\Space
+	  (lisp-code-print (car lisp-code-list))
+	  (lisp-code-print-help (cdr lisp-code-list)))))
+ 
+;; lisp-code-print: make printable lisp list
+(defun lisp-code-print (lisp-code)
+  "lisp-code-print: make a printable lisp code list"
+  (cond ((equal lisp-code 'nil) "nil") ;; 
+	((equal lisp-code 'quote) "'") ;; quote
+	((atom lisp-code) lisp-code)
+	((and (equal 2 (length lisp-code))
+	      (equal (car lisp-code) 'quote))
+	 (cons "'"
+	       (lisp-code-print (cadr lisp-code))))
+	(t
+	 (list '\(
+	  (cons (lisp-code-print (car lisp-code))
+		(lisp-code-print-help (cdr lisp-code)))
+	  '\) ))))
+)
+
+;; my-prove-SMT-formula
 (defun my-prove-SMT-formula (term)
+  "my-prove-SMT-formula: check if term is a valid SMT formula"
   (let ((decl-list (cadr (cadr term)))
 	(hypo-list (caddr (cadr term)))
 	(concl-list (caddr term)))
@@ -15,22 +45,65 @@
 		 hypo-list
 		 concl-list)))
 
+;; my-prove-write-file
 (defun my-prove-write-file (term fdir)
+  "my-prove-write-file: write translated term into a file"
   (write-SMT-file fdir
 		  (translate-SMT-formula
 		   (my-prove-SMT-formula term))
 		  state))
 
+;; my-prove-write-expander-file
+(defun my-prove-write-expander-file (expanded-term fdir)
+  "my-prove-write-expander-file: write expanded term into a log file"
+  (write-expander-file fdir
+		       expanded-term
+		       state))
+
+;; create-level
+(defun create-level (level index)
+  "create-level: creates a name for a level"
+  (intern-in-package-of-symbol
+   (concatenate 'string level (str::natstr index)) 'ACL2))
+
+;; my-prove-write-log-file
+(defun my-prove-write-log-file (expanded-term-list fdir index)
+  "my-prove-write-log-file: write the log file for expanding the functions"
+  (if (endp expanded-term-list)
+      t
+    (prog2$ (my-prove-write-expander-file
+	     (list (create-level "level" index) '\:  #\Newline
+		   (lisp-code-print
+		    (car expanded-term-list)))
+	     fdir)
+	    (my-prove-write-log-file
+	     (cdr expanded-term-list)
+	     fdir
+	     (1+ index)))))
+
+;; my-prove
 (defun my-prove (term fn-lst level fname)
+  "my-prove: return the result of calling SMT procedure"
   (let ((file-dir (concatenate 'string
 			       *dir-files*
 			       "/"
 			       fname
-			       ".py")))
-    (mv-let (expanded-term num)
+			       ".py"))
+	(expand-dir (concatenate 'string
+				 *dir-expanded*
+				 "/"
+				 fname
+				 "\_expand.log")))
+    (mv-let (expanded-term-list num)
 	    (expand-fn-top term fn-lst level state)
-	    (prog2$ (cw "~q0 ~%" expanded-term)
-		    (prog2$ (my-prove-write-file expanded-term file-dir)
+	    (prog2$ (cw "~q0 ~%" expanded-term-list)
+		    (prog2$ (my-prove-write-log-file
+			     expanded-term-list
+			     expand-dir
+			     0)
+			    (prog2$ (my-prove-write-file
+				     expanded-term-list
+				     file-dir)
 			    (if (car (SMT-interpreter file-dir))
-				(mv t expanded-term)
-			      (mv nil expanded-term)))))))
+				(mv t (my-last expanded-term-list))
+			      (mv nil (my-last expanded-term-list)))))))))
